PoS/Protocol.v
@@ -3,14 +3,12 @@ Require Import ssreflect ssrbool ssrnat eqtype ssrfun seq.
 From mathcomp
 Require Import path.
 Require Import Eqdep pred prelude idynamic ordtype pcm finmap unionmap heap coding.
-Require Import Blockchain.
+Require Import Blockchain BlockchainProperties.
 Set Implicit Arguments.
 Unset Strict Implicit.
 Unset Printing Implicit Defensive.
 
 (* Implementation of PoS protocol as a STS *)
-Parameter GenesisBlock : Block.
-
 Definition nid := nat.
 Definition peers_t := seq nid.
 
@@ -239,6 +237,41 @@ case=> n1 p1 b1 t1 a i []; do? by [].
 move=> p h. simpl. case exB: (ohead _). by [].
 case exT: (ohead _); by [].
 Qed.  
+
+Ltac local_bc_no_change s1 hbc hbc' :=
+  (rewrite /procMsg; destruct s1=>/=; rewrite /blockTree in hbc;
+     by move=>hbc'; rewrite hbc in hbc'; rewrite hbc';
+              apply or_introl; apply bc_pre_refl).
+
+Lemma procMsg_bc_prefix_or_fork bc bc':
+  forall (s1 : State) (m : Message), let: s2 := (procMsg s1 m).1 in
+    btChain (blockTree s1) = bc ->
+    btChain (blockTree s2) = bc' ->
+    [bc <<= bc'] \/ fork bc bc'.
+Proof.
+move=>s1; case =>[|p prs|p|b|t|p sh|p h] hbc; do? local_bc_no_change s1 hbc hbc'.
+- case: s1 hbc =>/= _ _ bt _ _ _ hbc. case B: (b \in bt).
+  by specialize (btExtend_withDup_noEffect B)=><-<-;
+     rewrite hbc; apply or_introl; apply bc_pre_refl.
+
+  move=>hbc'. rewrite -hbc -hbc'.
+  (* Extension – note that b is not necessarily the last block in bc' *)
+  case E: (prevBlockHash (bcLast bc') == hashB (bcLast bc)).
+  + apply or_introl.
+    move/negbT/btChain_mem in B. rewrite hbc in B.
+    specialize (btChain_extend hbc B E)=>->. rewrite hbc /is_prefix -cats1.
+    by exists [:: bcLast bc'].
+  (* Fork *)
+  + apply or_intror.
+    move/negbT/btChain_mem in B. rewrite hbc in B. rewrite -hbc' in E.
+    move/negbT in E. specialize (btChain_fork hbc B E)=> F.
+    by rewrite -hbc in F; apply F.
+- destruct s1=>/=. case (ohead _ ). rewrite /blockTree in hbc *=>/=.
+  + move=> _ hbc'. rewrite hbc in hbc'.
+    by rewrite -hbc'; apply or_introl; apply bc_pre_refl.
+  + case (ohead _) => [x hbc'|hbc']; rewrite /blockTree in hbc *=>/=;
+    by rewrite hbc in hbc'; rewrite -hbc'; apply or_introl; apply bc_pre_refl.
+Qed.
 
 Lemma procInt_peers_uniq :
   forall (s1 : State) (t : InternalTransition), let: s2 := (procInt s1 t).1 in
